Progress

liquid-copy/AVL.fst
@@ -10,22 +10,20 @@ let rec all_tree f = function
     | Leaf -> true
     | (Node k l r _) -> f k && all_tree f l && all_tree f r 
 
-val less_k : k:int -> x:int -> Tot bool
-let less_k k x = x < k 
-
-val more_k : k:int -> x:int -> Tot bool
-let more_k k x = x > k 
+val in_tree : x:int -> t:tree -> Tot bool
+let rec in_tree x = function
+  | Leaf -> false
+  | Node y l r _ -> y = x || in_tree x l || in_tree x r
 
 val all_more_than : k:int -> t:tree -> Tot bool
 let rec all_more_than k = function 
 | Leaf -> true
 | Node y l r _ -> y > k && all_more_than k l && all_more_than k r 
 
-val all_less_than : k:int -> t:tree -> Tot bool
+val all_less_than : k:int -> t:tree -> Tot (r:bool {r <==> (forall x. in_tree x t ==> x < k)})
 let rec all_less_than k = function 
 | Leaf -> true
 | Node y l r _ -> y < k && all_less_than k l && all_less_than k r 
-
 
 val is_bst : tree -> Tot bool
 let rec is_bst = function
@@ -113,10 +111,8 @@ let head (Node x _ _ _) = x
 val left: t:tree {not_empty t} -> Tot tree
 let left (Node _ l _ _) = l 
 
-
 val right: t:tree {not_empty t} -> Tot tree
 let right (Node _ _ r _) = r
-
 
 val left_of_avl_is_avll : t:avl{not_empty t} -> y:int {y == head t } -> Lemma(all_less_than y (left t))
 let left_of_avl_is_avll t y = ()
@@ -157,13 +153,11 @@ let is_left_big l r = diff l r = 2
 val is_right_big : l:tree{has_real_heights l} -> r:tree{has_real_heights r} -> Tot bool
 let is_right_big l r = diff r l = 2
 
+val all_more_transitive: v:int -> x:int {x > v} -> l:tree {all_more_than x l} -> Lemma (all_more_than v l)
+let all_more_transitive v x l = admit ()
 
-val all_more_intro_p: v:int -> x:int {x > v} -> l:tree {all_more_than x l} -> Lemma (all_more_than v l)
-let all_more_intro_p v x l = admit ()
-
-
-val all_less_intro_p: v:int -> x:int {x <= v} -> l:tree {all_less_than x l} -> Lemma (all_less_than v l)
-let all_less_intro_p v x l = admit ()
+val all_less_transitive: v:int -> x:int {x <= v} -> l:tree {all_less_than x l} -> Lemma (all_less_than v l)
+let all_less_transitive v x l = admit ()
 
 val all_more_intro: v:int -> x:int {x > v} -> l:avll x {all_more_than v l} -> r:avlr x{all_more_than v r && has_bal 1 l r} -> Lemma (all_more_than v (mk_node x l r))
 let all_more_intro v x l r  = ()
@@ -175,13 +169,13 @@ val balL0 : x:int -> l:avll x {is_not_heavy l} -> r:avlr x {is_left_big l r} -> 
 let balL0 x l r = match l with 
   | (Node lv ll lr _) -> 
     let y = mk_node x lr r in
-    all_more_intro_p lv x r;
+    all_more_transitive lv x r;
     mk_node lv ll y
   | _ -> admit ()
 
 val balLL : x:int -> l:avll x {is_left_heavy l} -> r:avlr x {is_left_big l r} -> avlt l
 let balLL v (Node lv ll lr _) r =
-  all_more_intro_p lv v r;
+  all_more_transitive lv v r;
   mk_node lv ll (mk_node v lr r)
 
 val eq_or_up : s:tree{has_real_heights s} -> t:tree{has_real_heights t} -> Tot bool
@@ -203,50 +197,49 @@ let big_ht l r t =
 val re_bal : l:tree {has_real_heights l} -> r:tree {has_real_heights r} -> t:tree{has_real_heights t} -> Tot bool  
 let re_bal l r t = big_ht l r t && bal_ht l r t
 
-val transitividad : a:int -> b:int {b > a} -> c:int {b < c} -> Lemma (a < c)
-let transitividad a b c = ()
-
 val balLR :x:int  -> l:avll x {is_right_heavy l} -> r:avlr x {is_left_big l r} -> Tot (avlt l)
 let balLR v l r = match l with
   | (Node lv ll (Node lrv lrl lrr lrh) lh) -> 
     let y = mk_node v lrr r in
        
-    all_more_intro_p lrv v r;
-    all_less_intro_p lrv lv ll; 
+    all_more_transitive lrv v r;
+    all_less_transitive lrv lv ll; 
 
     mk_node lrv (mk_node lv ll lrl) (y)
   | _ -> 
-    (* assert (! (is_right_heavy l)); *)
-    
+    (* should be impossible *)
     admit()
 
 
 val balR0 : x:int  -> r:avlr x {is_not_heavy r} -> l:avll x {is_right_big l r} -> Tot (avln (real_height r + 1))
 let balR0 x r l = match r with 
   | (Node rv rl rr _) ->
-    all_less_intro_p rv x l;
+    all_less_transitive rv x l;
     mk_node rv (mk_node x l rl) rr
   | _ -> 
+   (* should be impossible *)
     admit ()
 
 
 val balRR : x:int -> l:avll x -> r:avlr x {is_right_big l r && is_right_heavy r} -> Tot (avlt r)
 let balRR x l (Node rv rl rr _) = 
-  all_less_intro_p rv x l;
+  all_less_transitive rv x l;
   mk_node rv (mk_node x l rl) rr 
 
 val balRL : x:int -> l: avll x -> r:avlr x {is_right_big l r && is_left_heavy r} -> Tot (avlt r)
 let balRL x l = function
   | (Node rv (Node rlv rll rlr _) rr _) -> 
-    all_less_intro_p rlv x l;
-    all_more_intro_p rlv rv rr;
+    all_less_transitive rlv x l;
+    all_more_transitive rlv rv rr;
     mk_node rlv (mk_node x l rll ) (mk_node rv rlr rr)
   | _ -> 
     (* should be impossible *)
     admit ()
 
+
 val bal : x:int -> l:avll x -> r:avlr x {has_bal 2 l r} -> t:avl {re_bal l r t}
 let bal v l r  = 
+  admit ();
   let ilb = is_left_big l r in
   let irb = is_right_big l r in
   if (ilb && is_left_heavy l) then balLL v l r
@@ -276,7 +269,71 @@ let maximum_all_less_lemma t = admit ()
 val all_less_minimum_lemma : v:int -> t:tree{all_less_than v t} -> Lemma (not_empty t ==> maximum t < v)
 let all_less_minimum_lemma v t = admit ()
 
+val elems : t:tree -> Tot (Set.set int)
+let rec elems = function
+  | Leaf -> Set.empty
+  | Node x l r _ ->  Set.union (Set.singleton x) (Set.union (elems l)  (elems r))
 
+
+(*val add_elems_prop : x:int -> t:tree -> s:tree -> Tot logical  *)
+let add_elems_prop x t s = (forall y. (Set.mem y (elems s) ) <==> (y == x \/  (Set.mem y (elems t))))
+
+
+val elems_less_than_lemma : v:int -> t:tree {forall y. (Set.mem y (elems t) ==> y < v)} -> Lemma (all_less_than v t)
+let elems_less_than_lemma v t = admit ()
+
+val less_than_elems_lemma : v:int -> t:tree {all_less_than v t} -> Lemma (forall y. (Set.mem y (elems t) ==> y < v))
+let less_than_elems_lemma v t = admit ()
+
+
+let add_elems_in_tree x t s = (forall y. (in_tree y s ) ==> (y == x \/ (in_tree y t)))
+
+
+val in_tree_less_than_lemma : v:int -> t:tree {forall y. (in_tree y t ==> y < v)} -> Lemma (all_less_than v t)
+let in_tree_less_than_lemma v t = admit ()
+
+
+val in_tree_more_than_lemma : v:int -> t:tree {forall y. (in_tree y t ==> y > v)} -> Lemma (all_more_than v t)
+let in_tree_more_than_lemma v t = admit ()
+
+
+val less_than_in_tree_lemma : v:int -> t:tree {all_less_than v t} -> Lemma (forall y. (in_tree y t ==> y < v))
+let less_than_in_tree_lemma v t = admit ()
+
+
+val more_than_in_tree_lemma : v:int -> t:tree {all_more_than v t} -> Lemma (forall y. (in_tree y t ==> y > v))
+let more_than_in_tree_lemma v t = admit ()
+
+
+val insert_bst : x:int -> t:tree {is_bst t} -> Tot (r:tree {is_bst r /\ (forall y. in_tree y r <==> (in_tree y t \/ x = y))})
+let rec insert_bst x t =
+  match t with
+  | Leaf -> singleton x
+  | Node n t1 t2 _ -> if x = n then      t
+                    else if x < n then Node n (insert_bst x t1) t2 (node_height (insert_bst x t1) t2)
+                    else               begin
+                      more_than_in_tree_lemma n t2;
+                      in_tree_more_than_lemma n (insert_bst x t2);
+                      Node n t1 (insert_bst x t2) (node_height t1 (insert_bst x t2))
+                    end
+
+
+val insert: x:int -> s:avl -> Tot (t:avl {not_empty t /\ eq_or_up s t /\ (forall y. in_tree y t <==> (in_tree y s \/ x = y))})
+let rec insert x s = match s with
+  | Leaf -> singleton x
+  | Node v l r _ -> 
+    if x < v then begin
+      let insl = insert x l in
+      less_than_in_tree_lemma v l;
+      in_tree_less_than_lemma v insl;
+       
+      bal v insl r
+    end else if x > v then begin
+      admit ()
+    end else s
+
+
+(*
 val insert: x:int -> s:avl -> Tot (t:avl {not_empty t /\ eq_or_up s t /\ (minimum t = (if is_empty s then x else min x (minimum s))) /\ (maximum t = (if is_empty s then x else max x (maximum s)))}) (decreases s)
 let rec insert x t = match t with
   | (Node v l r n) ->
@@ -285,9 +342,10 @@ let rec insert x t = match t with
       all_less_minimum_lemma v l;
       assert (maximum insl <= v - 1);
       maximum_all_less_lemma insl;
-      all_less_intro_p v (maximum insl + 1) insl;
+      all_less_transitive v (maximum insl + 1) insl;
       bal v insl r
     end else if x > v then begin
       bal v l (insert x r)
     end else t
   | Leaf -> singleton x
+*)
